add lambda

benchmark/fibo.v
@@ -15,7 +15,7 @@ Fixpoint fib (n : nat) : int :=
         end
   end.
 
-Compute fib 10 10.
+Compute fib 10%nat.
 
 Theorem int_eq_spec:
   forall x y : int, reflect (x = y) (eqb x y).
@@ -25,38 +25,38 @@ Proof.
   + apply ReflectF. now apply eqb_false_spec.
 Qed.
 
-Module Int <: Hash_type.
-  Definition A := int.
-  Definition eq x y:= eqb x y.
-  Definition eq_spec := int_eq_spec.
-  Definition hash i: A := i.
-End Int.
-
-Module HashT := HashTable (Int).
-
-Fixpoint fib_memo' (n: nat) (m: int) (h: HashT.t nat) : nat * (HashT.t nat) :=
-  match HashT.find h m with
-  | Some v => (v, h)
-  | None =>
-      match n with
-      | 0 => (0, HashT.add h m 0)%nat
-      | S n' => 
-          match n' with
-          | 0 => (1, HashT.add h m 1)%nat
-          | S n'' => 
-              let (v1, h1) := fib_memo' n'  (m - 1) h  in
-              let (v2, h2) := fib_memo' n'' (m - 2) h1 in
-              let h3 := HashT.add h2 m (v1 + v2)%nat in
-              match HashT.find h3 m with
-              | Some v => (v, h3)
-              | None => (0, h3)%nat
-              end
-          end
-      end
-  end.
-
-Definition fib_memo n m := fst (fib_memo' n m (HashT.create Z 16)).
-
-Compute fib 35 35.
-
-Compute fib_memo 35 35.
+(* Module Int <: Hash_Type. *)
+(*   Definition A := int. *)
+(*   Definition eq x y:= eqb x y. *)
+(*   Definition eq_spec := int_eq_spec. *)
+(*   Definition hash i: A := i. *)
+(* End Int. *)
+(**)
+(* Module HashT := HashTable (Int). *)
+(**)
+(* Fixpoint fib_memo' (n: nat) (m: int) (h: HashT.t nat) : nat * (HashT.t nat) := *)
+(*   match HashT.find h m with *)
+(*   | Some v => (v, h) *)
+(*   | None => *)
+(*       match n with *)
+(*       | 0 => (0, HashT.add h m 0)%nat *)
+(*       | S n' =>  *)
+(*           match n' with *)
+(*           | 0 => (1, HashT.add h m 1)%nat *)
+(*           | S n'' =>  *)
+(*               let (v1, h1) := fib_memo' n'  (m - 1) h  in *)
+(*               let (v2, h2) := fib_memo' n'' (m - 2) h1 in *)
+(*               let h3 := HashT.add h2 m (v1 + v2)%nat in *)
+(*               match HashT.find h3 m with *)
+(*               | Some v => (v, h3) *)
+(*               | None => (0, h3)%nat *)
+(*               end *)
+(*           end *)
+(*       end *)
+(*   end. *)
+(**)
+(* Definition fib_memo n m := fst (fib_memo' n m (HashT.create Z 16)). *)
+(**)
+(* Compute fib 35 35. *)
+(**)
+(* Compute fib_memo 35 35. *)
