benchmark/lambda.v
@@ -1,0 +1,231 @@
+Require Import hashtable dict module utils.
+Require Import Nat ZArith Bool.
+Require Import Coq.Numbers.Cyclic.Int63.Uint63.
+Require Import Coq.Lists.List.
+Import ListNotations.
+
+Require Import quicksort.
+
+Open Scope uint63_scope.
+
+Module Term <: Hash_type.
+  Definition A := term.
+
+  Fixpoint eq n m :=
+    match n, m with
+    | Ref i, Ref j => i =? j
+    | Abs u, Abs v => eq u v
+    | App u1 u2, App v1 v2 => if eq u1 v1 then eq u2 v2 else false
+    | _, _ => false
+    end.
+
+  Lemma eqb_eq_refl:
+    forall n m, reflect (n = m) (eq n m).
+  Proof.
+    induction n; destruct m; simpl; try now apply ReflectF.
+    + case (i =? i0) eqn:H. apply eqb_spec in H. apply ReflectT. now rewrite H.
+      apply ReflectF. intros [= <-]. now rewrite eqb_refl in H.
+    + case (IHn m) as [<- | Hneq]. now apply ReflectT. apply ReflectF.
+      now intros [= <-].
+    + case (IHn1 m1) as [<- | H0]. case (IHn2 m2) as [<- | H1].
+      now apply ReflectT. all:apply ReflectF; now intros [= <-].
+  Qed.
+
+  Definition eq_spec := eqb_eq_refl.
+
+  Fixpoint hashi (t: term): int :=
+    match t with
+    | Ref i => i
+    | Abs t => (19 * hashi t + 1)
+    | App u v => (19 * (19 * hashi u + hashi v) + 2)
+    end.
+
+  Definition hashp (t: term): positive :=
+    let hi := hashi t in
+    match to_Z hi with
+    | Z.pos p => p
+    | _ => xH
+    end.
+End Term.
+
+Module Test (H: HashTable Term).
+
+  Record ht : Type := hash_tabs {
+    (* lift_h : H.t term; *)
+    (* subst_h : H.t term; *)
+    t_nf : H.t term;
+    t_hnf : H.t term;
+  }.
+
+  Definition memo_nf ht t nt :=
+    hash_tabs (H.add (t_nf ht) t nt) (t_hnf ht).
+
+  Definition memo_hnf ht t nt :=
+    hash_tabs (t_nf ht) (H.add (t_hnf ht) t nt).
+
+  Definition lift n :=
+    let lift_rec :=
+      fix lift_rec k t :=
+        match t with
+        | Ref i => if i <? k then t else Ref (n + i)
+        | Abs t => Abs (lift_rec (k + 1) t)
+        | App t u => App (lift_rec k t) (lift_rec k u)
+        end
+    in
+    lift_rec 0.
+
+  Definition subst w :=
+    let subst_w :=
+      fix subst_w n t :=
+        match t with
+        | Ref k =>
+          if k =? n then lift n w
+          else if k <? n then t
+          else Ref (k - 1)
+        | Abs t => Abs (subst_w (n + 1) t)
+        | App t u => App (subst_w n t) (subst_w n u)
+        end
+    in
+    subst_w 0.
+
+  Fixpoint fuell_hnf n t (ht : ht) :=
+    match H.find (t_hnf ht) t with
+    | Some t => (ht, t)
+    | None =>
+        match n, t with
+        | O, _ => (ht, t)
+        | S _, Ref n => (ht, t)
+        | S n, Abs t =>
+            let (ht, v) := fuell_hnf n t ht in
+            (memo_hnf ht t v, Abs v)
+        | S n, App t u =>
+            match fuell_hnf n t ht with
+            | (ht, Abs w) =>
+                let s := (subst u w) in
+                let (ht, v) := fuell_hnf n s ht in
+                (memo_hnf ht s v, v)
+                (* fuell_hnf n (subst u w) ht *)
+            | (ht, h) => (memo_hnf ht t h, App h u)
+            end
+        end
+    end.
+
+  Fixpoint fuell_nf n t (ht: ht) :=
+    match H.find (t_nf ht) t with
+    | Some t => (ht, t)
+    | None =>
+        match n, t with
+        | O, _ => (ht, t)
+        | S _, Ref n => (ht,t)
+        | S n, Abs t =>
+            let (ht, v) := fuell_nf n t ht in
+            (memo_nf ht t (Abs v), Abs v)
+        | S n, App t u =>
+            match fuell_hnf n t ht with
+            | (ht, Abs w) =>
+                let s := (subst u w) in
+                let (ht, v) := fuell_nf n s ht in
+                (memo_nf ht s v, v)
+            | (ht, h) =>
+                let (ht1, v1) := fuell_nf n h ht in
+                let ht2 := memo_nf ht1 h v1 in
+                let (ht3, v2) := fuell_nf n u ht2 in
+                (memo_nf ht u v2, App v1 v2)
+            end
+        end
+    end.
+
+  (* Definition hnf t := fuell_hnf 1000 t. *)
+  Definition nf t  :=
+    (fuell_nf 1000 t (hash_tabs (H.create 100) (H.create 100))).
+
+  Definition nil := (*[c,n]n*) Abs (Abs (Ref 0)).
+  Definition cons := (*[x,l][c,n](c x (l c n))*)
+    Abs (Abs (Abs (Abs (
+      App (App (Ref 1) (Ref 3))
+          (App (App (Ref 2) (Ref 1)) (Ref 0)))))).
+
+  Definition zero := Abs (Abs (Ref 0)).
+  Definition succ :=
+    Abs (Abs (Abs (
+      App (Ref 1)
+          (App (App (Ref 2) (Ref 1)) (Ref 0))))).
+
+  Definition church n :=
+    fold_int (fun _ t => snd (nf (App succ t)) ) n zero.
+
+  Fixpoint list l :=
+    match l with
+    | x :: l =>
+        let cx := church x in
+        let ll := list l in
+        (*[c,n](c x (l c n))*)
+        Abs (Abs (App (App (Ref 1) cx)
+          (App (App ll (Ref 1)) (Ref 0))))
+    | [] => nil
+    end.
+
+  (* Back *)
+
+  Fixpoint eval_iter {T: Type} (iter: option T -> option T) init t :=
+    match t with
+    | Ref i => if i =? 0 then init else None
+    | App (Ref i) u =>
+        if i =? 1
+        then iter (eval_iter iter init u)
+        else None
+    | _ => None
+    end.
+
+  Definition compute_nat t :=
+    match t with
+    | Abs (Abs t) =>
+        eval_iter
+          (fun i =>
+            match i with
+            | Some i => Some (i+1)
+            | None => None end)
+          (Some 0) t
+    | _ => None
+    end.
+
+  Definition eval_list_of_nats t :=
+    match t with
+    | Abs (Abs t) =>
+        let lrec :=
+          fix lrec t :=
+            match t with
+            | Ref i => if i =? 0 then Some [] else None
+            | App (App (Ref i) x) l =>
+                if i =? 1 then
+                  match compute_nat x, lrec l with
+                  | Some x, Some ll => Some (x :: ll)
+                  | _, _ => None
+                  end
+                else None
+            | _ => None
+            end
+        in
+        lrec t
+    | _ => None
+    end.
+
+  Definition normal_nat n := compute_nat (snd (nf n)).
+  Definition normal_list l := 
+    let (ht, t) := nf l in
+    (ht, eval_list_of_nats t).
+
+End Test.
+
+
+(* bench *)
+Module HTree := HashTableTree Term.
+Module TestTree := Test HTree.
+
+Module HBucket := HashTableBucket Term.
+Module TestBucket := Test HBucket.
+
+Definition l := TestBucket.list [0].
+Time Compute TestTree.normal_list (App quicksort l).
+Time Compute TestBucket.normal_list (App quicksort l).
+
