benchmark/quicksort.v
@@ -1,0 +1,125 @@
+Require Import Coq.Numbers.Cyclic.Int63.Uint63.
+
+Inductive term :=
+  | Ref : int -> term
+  | Abs : term -> term
+  | App : term -> term -> term.
+
+Definition quicksort := App (App (Abs (Abs (App (Ref 0) (App (App (Ref 1) (Ref 1)) (Ref 0)))))
+     (Abs (Abs (App (Ref 0) (App (App (Ref 1) (Ref 1)) (Ref 0))))))
+(Abs
+ (App (Abs (Abs (App (App (Ref 0) (Ref 1)) (Abs (Abs (Ref 0))))))
+  (Abs
+   (Abs
+    (App (Abs
+          (App (App (Abs
+                     (Abs
+                      (Abs
+                       (Abs
+                        (App (App (Ref 3) (Ref 1))
+                         (App (App (Ref 2) (Ref 1)) (Ref 0)))))))
+                (App (Ref 3)
+                 (App (Abs (App (Ref 0) (Abs (Abs (Ref 1))))) (Ref 0))))
+           (App (App (Abs
+                      (Abs
+                       (Abs
+                        (Abs
+                         (App (App (Ref 1) (Ref 3))
+                          (App (App (Ref 2) (Ref 1)) (Ref 0)))))))
+                 (Ref 2))
+            (App (Ref 3)
+             (App (Abs (App (Ref 0) (Abs (Abs (Ref 0))))) (Ref 0))))))
+     (App (App (Abs
+                (Abs
+                 (App (Abs
+                       (App (App (Ref 1) (Ref 0))
+                        (App (App (Abs
+                                   (Abs
+                                    (Abs (App (App (Ref 0) (Ref 2)) (Ref 1)))))
+                              (Abs (Abs (Ref 0))))
+                         (Abs (Abs (Ref 0))))))
+                  (Abs
+                   (Abs
+                    (App (Abs
+                          (App (Abs
+                                (App (App (App (Ref 5) (Ref 3))
+                                      (App (App (Abs
+                                                 (Abs
+                                                  (Abs
+                                                   (App (App (Ref 0) (Ref 2))
+                                                    (Ref 1)))))
+                                            (App (App (Abs
+                                                       (Abs
+                                                        (Abs
+                                                         (Abs
+                                                          (App (App (
+                                                                Ref 1)
+                                                                (Ref 3))
+                                                           (App (App (
+                                                                 Ref 2)
+                                                                 (Ref 1))
+                                                            (Ref 0)))))))
+                                                  (Ref 3))
+                                             (Ref 1)))
+                                       (Ref 0)))
+                                 (App (App (Abs
+                                            (Abs
+                                             (Abs
+                                              (App (App (Ref 0) (Ref 2))
+                                               (Ref 1)))))
+                                       (Ref 1))
+                                  (App (App (Abs
+                                             (Abs
+                                              (Abs
+                                               (Abs
+                                                (App (App (Ref 1) (Ref 3))
+                                                 (App (App (Ref 2) (Ref 1))
+                                                  (Ref 0)))))))
+                                        (Ref 3))
+                                   (Ref 0)))))
+                           (App (Abs (App (Ref 0) (Abs (Abs (Ref 0)))))
+                            (Ref 1))))
+                     (App (Abs (App (Ref 0) (Abs (Abs (Ref 1))))) (Ref 0))))))))
+           (App (Abs
+                 (Abs
+                  (App (App (App (App (Ref 1)
+                                  (App (Abs
+                                        (Abs
+                                         (App (Abs
+                                               (App (Ref 0)
+                                                (Abs (Abs (Ref 0)))))
+                                          (App (App (Ref 0) (Ref 1))
+                                           (App (App (Abs
+                                                      (Abs
+                                                       (Abs
+                                                        (App (App (Ref 0)
+                                                              (Ref 2))
+                                                         (Ref 1)))))
+                                                 (Abs (Abs (Ref 0))))
+                                            (Abs (Abs (Ref 0))))))))
+                                   (Abs
+                                    (App (Abs
+                                          (App (App (Abs
+                                                     (Abs
+                                                      (Abs
+                                                       (App (App (Ref 0)
+                                                             (Ref 2))
+                                                        (Ref 1)))))
+                                                (App (Abs
+                                                      (Abs
+                                                       (Abs
+                                                        (App (Ref 1)
+                                                         (App (App (Ref 2)
+                                                               (Ref 1))
+                                                          (Ref 0))))))
+                                                 (Ref 0)))
+                                           (Ref 0)))
+                                     (App (Abs
+                                           (App (Ref 0) (Abs (Abs (Ref 1)))))
+                                      (Ref 0))))))
+                             (Ref 0))
+                        (App (Abs (Abs (Ref 1))) (Abs (Abs (Ref 0)))))
+                   (Abs (Abs (Ref 1))))))
+            (Ref 1)))
+      (Ref 0))))))).
+
